compiler1/stack_namesScript.sml
@@ -50,4 +50,30 @@ val prog_comp_def = Define `
 val compile_def = Define `
   compile f prog = MAP (prog_comp f) prog`;
 
+(* some defaults *)
+
+val x64_names_def = Define `
+  x64_names =
+    (* 16 regs, must avoid 4 and 5, names:
+         r0=rax, r1=rbx, r2=rcx, r3=rdx, r4=rbp, r5=rsp, r6=rsi,
+         r7=rdi, r8=r8, r9, r10, r11, r12, r13, r14, r15
+       The first six arguments are passed in registers. The first
+       argument (1) is passed in rdi(r7), the second(2) in rsi(r6),
+       the third(3) in rdx(r3), the fourth(4) in rcx(2), the fifth(5)
+       in r8 and the sixth in r9.
+     *)
+    (insert 1 7 o
+     insert 2 6 o
+  (* insert 3 3 o *)
+     insert 4 2 o
+     insert 5 8 o
+     insert 6 9 o
+     (* the rest just ensures that the mapping is well-formed *)
+     insert 7 1 o
+     insert 8 14 o
+     insert 9 15) LN`
+
+val x64_names_def = save_thm("x64_names_def",
+  CONV_RULE (RAND_CONV EVAL) x64_names_def);
+
 val _ = export_theory();
